add bn_mod_exp_mont_ladder

code/bignum/Hacl.Bignum.Exponentiation.fst
@@ -9,11 +9,14 @@ open Lib.Buffer
 
 module BN = Hacl.Bignum
 module BM = Hacl.Bignum.Montgomery
+module BL = Hacl.Bignum.Lib
 
 open Hacl.Bignum.Definitions
 
 module ST = FStar.HyperStack.ST
 module S = Hacl.Spec.Bignum.Exponentiation
+module LSeq = Lib.Sequence
+module Loops = Lib.LoopCombinators
 
 friend Hacl.Spec.Bignum.Exponentiation
 
@@ -36,7 +39,7 @@ let bn_mod_exp_loop_st (nLen: BN.meta_len) =
     disjoint accM b /\ disjoint accM n)
   (ensures  fun h0 _ h1 -> modifies (loc aM |+| loc accM) h0 h1 /\
     (as_seq h1 aM, as_seq h1 accM) ==
-      Lib.LoopCombinators.repeati (v bBits)
+      Loops.repeati (v bBits)
 	(S.bn_mod_exp_f (as_seq h0 n) nInv_u64 (v bBits) (v bLen) (as_seq h0 b))
       (as_seq h0 aM, as_seq h0 accM))
 
@@ -51,7 +54,7 @@ let bn_mod_exp_loop nLen #_ n nInv_u64 bBits bLen b aM accM =
   let h0 = ST.get () in
   loop2 h0 bBits aM accM spec
   (fun i ->
-    Lib.LoopCombinators.unfold_repeati (v bBits) (spec h0) (as_seq h0 aM, as_seq h0 accM) (v i);
+    Loops.unfold_repeati (v bBits) (spec h0) (as_seq h0 aM, as_seq h0 accM) (v i);
     let get_bit = BN.bn_get_ith_bit bLen b i in
 
     if FStar.UInt64.(Lib.RawIntTypes.u64_to_UInt64 get_bit =^ 1uL) then
@@ -119,3 +122,122 @@ let bn_mod_exp_loop_runtime nLen = bn_mod_exp_loop nLen #(BM.mk_runtime_mont nLe
 [@CInline]
 let bn_mod_exp modBits nLen =
   mk_bn_mod_exp modBits nLen #(BM.mk_runtime_mont nLen) (bn_mod_exp_loop_runtime nLen)
+
+
+///
+///  Montgomery ladder for exponentiation
+///
+
+inline_for_extraction noextract
+let bn_mod_exp_mont_ladder_loop_st (nLen: BN.meta_len) =
+    n:lbignum nLen
+  -> nInv_u64:uint64
+  -> bBits:size_t{v bBits > 0}
+  -> bLen:size_t{v bLen = v (blocks bBits 64ul) /\ (v bBits - 1) / 64 < v bLen}
+  -> b:lbignum bLen
+  -> rM0:lbignum nLen
+  -> rM1:lbignum nLen
+  -> sw:lbignum 1ul ->
+  Stack unit
+  (requires fun h ->
+    live h n /\ live h b /\ live h rM0 /\ live h rM1 /\ live h sw /\
+    disjoint rM0 rM1 /\ disjoint rM0 b /\ disjoint rM0 n /\
+    disjoint rM1 b /\ disjoint rM1 n /\
+    disjoint sw rM0 /\ disjoint sw rM1 /\ disjoint sw b /\ disjoint sw n)
+  (ensures  fun h0 _ h1 -> modifies (loc rM0 |+| loc rM1 |+| loc sw) h0 h1 /\
+    (as_seq h1 rM0, as_seq h1 rM1, LSeq.index (as_seq h1 sw) 0) ==
+      Loops.repeat_gen (v bBits) (S.bn_mod_exp_mont_ladder_t (v nLen) (v bBits))
+	(S.bn_mod_exp_mont_ladder_f (as_seq h0 n) nInv_u64 (v bBits) (v bLen) (as_seq h0 b))
+      (as_seq h0 rM0, as_seq h0 rM1, LSeq.index (as_seq h0 sw) 0))
+
+inline_for_extraction noextract
+val bn_mod_exp_mont_ladder_loop: nLen:BN.meta_len
+  -> (#[FStar.Tactics.Typeclasses.tcresolve ()] _ : Hacl.Bignum.Montgomery.mont nLen)
+  -> bn_mod_exp_mont_ladder_loop_st nLen
+
+let bn_mod_exp_mont_ladder_loop nLen #_ n nInv_u64 bBits bLen b rM0 rM1 sw =
+  [@inline_let]
+  let refl h i : GTot (S.bn_mod_exp_mont_ladder_t (v nLen) (v bBits) i) =
+    (as_seq h rM0, as_seq h rM1, LSeq.index (as_seq h sw) 0) in
+  [@inline_let]
+  let footprint i = loc rM0 |+| loc rM1 |+| loc sw in
+  [@inline_let]
+  let spec h0 = S.bn_mod_exp_mont_ladder_f #(v nLen) (as_seq h0 n) nInv_u64 (v bBits) (v bLen) (as_seq h0 b) in
+  let h0 = ST.get () in
+  loop h0 bBits (S.bn_mod_exp_mont_ladder_t (v nLen) (v bBits)) refl footprint spec
+  (fun i ->
+    Loops.unfold_repeat_gen (v bBits) (S.bn_mod_exp_mont_ladder_t (v nLen) (v bBits)) (spec h0) (refl h0 0) (v i);
+    let bit = BN.bn_get_ith_bit bLen b (bBits -! i -! 1ul) in
+    let sw1 = bit ^. sw.(0ul) in
+    BL.cswap2_st nLen sw1 rM0 rM1;
+    BM.mul n nInv_u64 rM1 rM0 rM1;
+    BM.sqr n nInv_u64 rM0 rM0;
+    sw.(0ul) <- bit
+  );
+  let h1 = ST.get () in
+  assert (refl h1 (v bBits) == Loops.repeat_gen (v bBits) (S.bn_mod_exp_mont_ladder_t (v nLen) (v bBits)) (spec h0) (refl h0 0))
+
+
+inline_for_extraction noextract
+val bn_mod_exp_mont_ladder_:
+    modBits:size_t{v modBits > 0}
+  -> nLen:size_t{0 < v nLen /\ 128 * v nLen <= max_size_t /\ v nLen == v (blocks modBits 64ul)}
+  -> (#[FStar.Tactics.Typeclasses.tcresolve ()] _ : Hacl.Bignum.Montgomery.mont nLen)
+  -> bn_mod_exp_mont_ladder_loop:bn_mod_exp_mont_ladder_loop_st nLen
+  -> n:lbignum nLen
+  -> a:lbignum nLen
+  -> acc:lbignum nLen
+  -> bBits:size_t{v bBits > 0}
+  -> b:lbignum (blocks bBits 64ul)
+  -> res:lbignum nLen ->
+  Stack unit
+  (requires fun h ->
+    live h n /\ live h a /\ live h b /\ live h res /\ live h acc /\
+    disjoint res a /\ disjoint res b /\ disjoint res n /\ disjoint res acc /\
+    disjoint a n /\ disjoint acc n)
+  (ensures  fun h0 _ h1 -> modifies (loc res) h0 h1 /\
+    as_seq h1 res ==
+      S.bn_mod_exp_mont_ladder_ (v modBits) (v nLen) (as_seq h0 n) (as_seq h0 a) (as_seq h0 acc) (v bBits) (as_seq h0 b))
+
+let bn_mod_exp_mont_ladder_ modBits nLen #_ bn_mod_exp_mont_ladder_loop n a one bBits b res =
+  push_frame ();
+  let bLen = blocks bBits 64ul in
+  let nInv_u64 = BM.mod_inv_u64 n.(0ul) in // n * nInv = 1 (mod (pow2 64))
+
+  let r2 = create nLen (u64 0) in
+  BM.precomp modBits n r2;
+
+  let rM0 = create nLen (u64 0) in
+  let rM1 = create nLen (u64 0) in
+  let sw  = create 1ul (u64 0) in
+  BM.to n nInv_u64 r2 one rM0;
+  BM.to n nInv_u64 r2 a rM1;
+
+  bn_mod_exp_mont_ladder_loop n nInv_u64 bBits bLen b rM0 rM1 sw;
+  BL.cswap2_st nLen sw.(0ul) rM0 rM1;
+  BM.from n nInv_u64 rM0 res;
+  pop_frame ()
+
+
+inline_for_extraction noextract
+val mk_bn_mod_exp_mont_ladder:
+    modBits:size_t{v modBits > 0}
+  -> nLen:size_t{0 < v nLen /\ 128 * v nLen <= max_size_t /\ v nLen == v (blocks modBits 64ul)}
+  -> (#[FStar.Tactics.Typeclasses.tcresolve ()] _ : Hacl.Bignum.Montgomery.mont nLen)
+  -> bn_mod_exp_mont_ladder_loop:bn_mod_exp_mont_ladder_loop_st nLen ->
+  bn_mod_exp_mont_ladder_st modBits nLen
+
+let mk_bn_mod_exp_mont_ladder modBits nLen #_ bn_mod_exp_mont_ladder_loop n a bBits b res =
+  push_frame ();
+  let one  = create nLen (u64 0) in
+  BN.bn_from_uint nLen (u64 1) one;
+  bn_mod_exp_mont_ladder_ modBits nLen bn_mod_exp_mont_ladder_loop n a one bBits b res;
+  pop_frame ()
+
+/// A fully runtime implementation of modular exponentiation.
+
+let bn_mod_exp_mont_ladder_loop_runtime nLen = bn_mod_exp_mont_ladder_loop nLen #(BM.mk_runtime_mont nLen)
+
+[@CInline]
+let bn_mod_exp_mont_ladder modBits nLen =
+  mk_bn_mod_exp_mont_ladder modBits nLen #(BM.mk_runtime_mont nLen) (bn_mod_exp_mont_ladder_loop_runtime nLen)
