code/bignum/Hacl.Spec.Bignum.Exponentiation.fsti
@@ -10,7 +10,7 @@ open Hacl.Spec.Bignum.Definitions
 
 #reset-options "--z3rlimit 50 --fuel 0 --ifuel 0"
 
-// This functions is *NOT* constant-time on the exponent b
+// This function is *NOT* constant-time on the exponent b
 val bn_mod_exp:
     modBits:size_pos
   -> nLen:size_pos{nLen = blocks modBits 64 /\ 128 * nLen <= max_size_t}
@@ -36,7 +36,7 @@ val bn_mod_exp_lemma:
     bn_v (bn_mod_exp modBits nLen n a bBits b) == Lib.NatMod.pow_mod #(bn_v n) (bn_v a) (bn_v b))
 
 
-// This functions is constant-time on the exponent b
+// This function is constant-time on the exponent b
 val bn_mod_exp_mont_ladder:
     modBits:size_pos
   -> nLen:size_pos{nLen = blocks modBits 64 /\ 128 * nLen <= max_size_t}
